src/Distributions/UniformPowerOfTwo/Implementation.dfy
@@ -12,13 +12,15 @@ module UniformPowerOfTwoImplementation {
 
   trait {:termination false} Trait extends Interface.Trait {
     method UniformPowerOfTwoSample(n: nat) returns (u: nat)
+      requires n >= 1
       modifies this
       ensures Model.Sample(n)(old(s)) == (u, s)
     {
       u := 0;
       var n' := n;
 
-      while n' > 0
+      while n' > 1
+        invariant n' >= 1
         invariant Model.SampleTailRecursive(n)(old(s)) == Model.SampleTailRecursive(n', u)(s)
       {
         var b := CoinSample();
