src/Distributions/UniformPowerOfTwo/Interface.dfy
@@ -12,7 +12,9 @@ module UniformPowerOfTwoInterface {
 
   trait {:termination false} Trait extends Coin.Interface.Trait {
 
+    // The return value u is uniformly distributed between 0 <= u < 2^k where 2^k <= n < 2^(k + 1).
     method UniformPowerOfTwoSample(n: nat) returns (u: nat)
+      requires n >= 1
       modifies this
       ensures Model.Sample(n)(old(s)) == (u, s)
 
